progress

src/Examples/HA/SampleProofs.v
@@ -15,6 +15,48 @@ Require Import IFOL.Examples.HA.Semantics.Sort.
 Require Import IFOL.Examples.HA.Semantics.Signature.
 Require Import IFOL.Examples.HA.Semantics.Theory.
 
+Definition plus_commutes_aux :
+  Formula HA_sig (Nat :: nil).
+Proof.
+  apply (QuantifierProp _ Nat Pi).
+  apply (EqualityProp _ _ Nat).
+  - apply (@f_app _ HA_f_sig _ Plus).
+    + apply hvcons.
+      * exact (var _ (wtl whd)).
+      * apply hvcons.
+        ** exact (var _ whd).
+        ** exact hvnil.
+  - apply (@f_app _ HA_f_sig _ Plus).
+    + apply hvcons.
+      * exact (var _ whd).
+      * apply hvcons.
+        ** exact (var _ (wtl whd)).
+        ** exact hvnil.
+Defined.
+
+Definition plus_commutes :
+  Formula HA_sig nil.
+Proof.
+  apply (QuantifierProp _ Nat Pi).
+  exact plus_commutes_aux.
+Defined.
+
+Lemma plus_commutes_pf :
+  @Proof _ _ HA_theory nil nil plus_commutes.
+Proof.
+  apply Pi_intro.
+  pose proof (@Ax _ _ HA_theory
+    (Induction plus_commutes_aux)
+    (Nat :: nil)
+    (BList.bump Nat (nil : BList.BList _ nil))
+  ) as ind_pf.
+  simpl in *.
+  apply 
+  simpl suff_weaken in ind_pf.
+  simpl in *.
+
+Admitted.
+
 Definition all_even_or_odd_aux :
   Formula HA_sig (Nat :: nil).
 Proof.
@@ -93,14 +135,171 @@ Proof.
       as pi_zplus.
     simpl in pi_zplus.
     unfold Zero_Plus_formula in pi_zplus.
-    epose Pi_elim.
     simpl in pi_zplus.
     unfold suff_weaken in pi_zplus.
     simpl in pi_zplus.
     exact (Pi_elim _ _ _ pi_zplus Z).
   }
-  epose proof
+  pose proof
     (Exp_elim HA_theory _ _ ind_pf P0) as p.
   simpl in p.
+  eapply Exp_elim.
+  exact p.
+  simpl.
+  apply Pi_intro.
+  simpl.
+  apply Exp_intro.
+  simpl.
+  assert
+    (@Proof _ _ HA_theory (Nat :: nil)%list
+ ((all_even_or_odd_aux :: nil)%list, nil)
+    all_even_or_odd_aux).
+pose (i := (inl (inl tt) : (@BList.bindex _ _ (Nat :: nil)%list
+((all_even_or_odd_aux :: nil)%list, nil)
+))).
+  exact (Assumption
+    HA_theory i
+  ).
+  apply (Sigma_elim _ _ _ _ X).
+  simpl.
+  pose ((inl (inl tt)) : (@BList.bindex _ _ (Nat :: Nat :: nil)%list
+((BinProp HA_sig Sum
+      (EqualityProp HA_sig (Nat :: Nat :: nil) Nat
+         (@f_app HA_sort HA_f_sig _ Plus
+            (hvcons (var Nat whd)
+               (hvcons (var Nat whd) hvnil)))
+         (var Nat (wtl whd)))
+      (EqualityProp HA_sig (Nat :: Nat :: nil) Nat
+         (@f_app HA_sort HA_f_sig _ Succ
+            (hvcons
+               (@f_app HA_sort HA_f_sig _ Plus
+                  (hvcons (var Nat whd)
+                     (hvcons (var Nat whd) hvnil)))
+               hvnil)) (var Nat (wtl whd))) :: nil)%list,
+   ((all_even_or_odd_aux :: nil)%list, nil))
+  )) as i.
+  pose proof (Assumption HA_theory i).
+  apply (Sum_elim _ _ _ _ X0).
+  + clear X0 i p P0 ind_pf.
+    simpl.
+    apply (Sigma_intro
+      HA_theory Nat _ (var Nat whd)).
+    apply Sum_intro_r.
+    simpl.
+    unfold eq_rect_r.
+    unfold eq_rect.
+    simpl.
+    pose (inl eq_refl : witness Nat (Signature.f_args
+      (@Signature.f_arities _ HA_f_sig Succ))).
+    unshelve epose (_ : (Formula_subterm_witness 
+(@f_app _ (Signature.func HA_sig) _ Plus
+                          (hvcons 
+                             (var Nat whd)
+                             (hvcons
+                                (var Nat whd)
+                                hvnil)))
+  (EqualityProp HA_sig
+                 (Nat :: Nat :: nil) Nat
+                 (@f_app _ HA_f_sig _ Succ
+                    (hvcons
+                       (@f_app _ HA_f_sig _ Plus
+                          (hvcons 
+                             (var Nat whd)
+                             (hvcons
+                                (var Nat whd)
+                                hvnil))) hvnil))
+                 (@f_app _ HA_f_sig _ Succ
+                    (hvcons
+                       (var Nat
+                         (wtl whd))
+                       hvnil))))
+    ).
+    { apply subterm_Equality_left.
+      apply (subterm_app w).
+      apply subterm_refl.
+    }
+    eapply (Eq_elim _ _ _ _ f).
+    * apply Eq_intro.
+    * simpl.
+      unshelve epose (_ : BList.BList (Formula HA_sig) (Nat :: Nat :: nil)).
+      { exact
+        ((EqualityProp HA_sig
+      (Nat :: Nat :: nil) Nat
+      (@f_app _ HA_f_sig _ Plus
+         (hvcons (var Nat whd)
+            (hvcons (var Nat whd) hvnil)))
+      (var Nat (wtl whd))
+    :: BinProp HA_sig Sum
+         (EqualityProp HA_sig
+            (Nat :: Nat :: nil) Nat
+            (@f_app _ HA_f_sig _ Plus
+               (hvcons (var Nat whd)
+                  (hvcons (var Nat whd)
+                     hvnil)))
+            (var Nat (wtl whd)))
+         (EqualityProp HA_sig
+            (Nat :: Nat :: nil) Nat
+            (@f_app _ HA_f_sig _ Succ
+               (hvcons
+                  (@f_app _ HA_f_sig _ Plus
+                     (hvcons
+                        (var Nat whd)
+                        (hvcons
+                          (var Nat whd)
+                          hvnil))) hvnil))
+            (var Nat (wtl whd))) :: nil)%list,
+   ((all_even_or_odd_aux :: nil)%list,
+    nil)). }
+    pose (i := inl (inl tt) : BList.bindex b).
+    exact (Assumption HA_theory i).
+  + clear X0 i p P0 ind_pf.
+    simpl.
+    apply (Sigma_intro
+      HA_theory Nat _
+      (@f_app HA_sort HA_f_sig _ Succ
+        (hvcons (var Nat whd) hvnil)
+      )).
+    apply Sum_intro_l.
+    simpl.
+    unfold eq_rect_r.
+    unfold eq_rect.
+    simpl.
+    unshelve epose (_ : Formula_subterm_witness
+      (@f_app _ (Signature.func HA_sig) _ Plus
+        (hvcons _
+          (hvcons _ hvnil)))
+(EqualityProp HA_sig
+     (Nat :: Nat :: nil) Nat
+     (@f_app _ HA_f_sig _ Plus
+        (hvcons
+           (@f_app _ HA_f_sig _ Succ
+              (hvcons (var Nat whd)
+                 hvnil))
+           (hvcons
+              (@f_app _ HA_f_sig _ Succ
+                 (hvcons (var Nat whd)
+                    hvnil)) hvnil)))
+     (@f_app _ HA_f_sig _ Succ 
+        (hvcons
+           (var Nat (wtl whd))
+           hvnil)))).
+    3:{ apply subterm_Equality_left.
+        apply subterm_refl.
+      }
+    eapply (Eq_elim _ _ _ _ f).
+    2:{ epose (sp :=
+      @Ax _ _ HA_theory Succ_Plus (Nat :: Nat :: nil) _).
+    simpl in sp.
+    unfold Succ_Plus_formula in sp.
+    simpl in sp.
+    pose (sp1 := Pi_elim _ _ _ sp (var Nat whd)).
+    pose (sp2 := Pi_elim _ _ _ sp1 (var Nat (wtl whd))).
+    simpl in sp2.
+    unfold eq_rect_r in sp2.
+    unfold eq_rect in sp2.
+    simpl in sp2.
+    exact sp2.
+q 
+  }
   admit.
 Admitted.
